not done

myex/Example_state.thy
@@ -8,10 +8,10 @@ record state =
   
 locale foo
   =
-  fixes Red :: "'a state_scheme"
+  fixes Rec :: "'a state_scheme"
 begin
   
-lemmas r_surj = state.surjective[of Red,symmetric]
+lemmas r_surj = state.surjective[of Rec,symmetric]
   
 lemmas foo = 
   state.update_convs[of "\<lambda>_. X" for X, @ (schematic) \<open>subst (asm) r_surj\<close>,symmetric]
@@ -19,6 +19,7 @@ lemmas foo =
 lemmas foo' = state.select_convs(1) select_convs
   
 lemmas foos = foo'[@ (schematic) \<open>subst (asm) foo(1)\<close>]
+              foo'[@ (schematic) \<open>subst (asm) foo(2)\<close>]
   
 end
   
